theories/Pi/Interpretation.v
@@ -2,11 +2,13 @@
 (*   Copyright (c) 2019--2024 - Paulo Torrens <paulotorrens AT gnu DOT org>   *)
 (******************************************************************************)
 
+Require Import Lia.
 Require Import Equality.
 Require Import Local.Prelude.
 Require Import Local.Substitution.
 Require Import Local.Syntax.
 Require Import Local.TypeSystem.
+Require Import Local.Pi.Graph.
 Require Import Local.Pi.Calculus.
 Require Import Local.Pi.Control.
 
@@ -14,20 +16,19 @@ Section Interpretation.
 
   Variable pi_base: type.
 
+  Hypothesis pi_base_is_output: alternating O pi_base.
+
   Definition is_variable (k: pseudoterm) (n: nat): Prop :=
     k = bound n.
-
-  Definition local_env p ts q :=
-    restriction (channel O ts)
-      (parallel p (replication 0 ts q)).
 
   Inductive interpret_type: pseudoterm -> type -> Prop :=
     | interpret_type_base:
       interpret_type base pi_base
     | interpret_type_negation:
-      forall ts cs,
+      forall ts cs t,
       Forall2 interpret_type ts cs ->
-      interpret_type (negation ts) (channel O cs).
+      t = dual (channel I cs) ->
+      interpret_type (negation ts) t.
 
   Inductive interpret: pseudoterm -> term -> Prop :=
     | interpret_jump:
@@ -40,7 +41,7 @@ Section Interpretation.
       interpret b p ->
       interpret c q ->
       Forall2 interpret_type ts cs ->
-      q' = (lift 1 (length cs) q) ->
+      q' = lift 1 (length cs) q ->
       interpret (bind b ts c) (local_env p cs q').
 
   Local Notation pB := (pi_base).
@@ -51,23 +52,116 @@ Section Interpretation.
     (* TODO: give an example number here. *)
     let p :=
       (* \j.\x.\y.\z.
-           (\h)((\k)(1<y@3, k@0, x@4>
-                   | !k@0(a, b).3<b@0, j@7, a@1>)
-              | !h@0(c, d, e).1<e@0, z@4>) *)
+           (\h)((\k)(h@1<y@3, k@0, x@4>
+                   | !k@0(a, b).h@3<b@0, j@7, a@1>)
+              | !h@0(c, d, e).d@1<e@0, z@4>) *)
       (restriction
-        (cO [pB; cO [pB; pB]; pB])
+        (cI [pB; cO [dual pB; dual pB]; pB])
         (parallel
-          (restriction (cO [pB; pB])
+          (restriction
+            (cI [pB; pB])
             (parallel
               (output 1 [4; 0; 3])
-              (replication 0 [pB; pB]
+              (replication 0
+                [pB; pB]
                 (output 3 [1; 7; 0]))))
-          (replication 0 [pB; cO [pB; pB]; pB]
-            (output 1 [4; 0])))) in
-    interpret Syntax.ex1 p.
+          (replication 0
+            [pB; cO [dual pB; dual pB]; pB]
+            (output 1 [4; 0]))))
+    in interpret Syntax.ex1 p.
   Proof.
-    compute.
     repeat econstructor.
   Qed.
+
+  Lemma interpret_generates_output:
+    forall t c,
+    interpret_type t c ->
+    alternating O c.
+  Proof.
+    fix H 3.
+    destruct 1.
+    - apply pi_base_is_output.
+    - subst; simpl.
+      constructor.
+      induction H0; simpl.
+      + constructor.
+      + constructor; auto.
+        replace I with (inverse O) by auto.
+        apply alternating_inverse_dual.
+        now apply H with x.
+  Qed.
+
+  Lemma interpret_forall_generates_output:
+    forall ts cs,
+    Forall2 interpret_type ts cs ->
+    Forall (alternating O) cs.
+  Proof.
+    induction 1; simpl.
+    - constructor.
+    - constructor; auto.
+      now apply interpret_generates_output with x.
+  Qed.
+
+  Inductive interpret_env: list pseudoterm -> env -> Prop :=
+    | interpret_env_nil:
+      interpret_env [] empty
+    | interpret_env_cons:
+      forall t ts c cs,
+      interpret_type t c ->
+      interpret_env ts cs ->
+      interpret_env (t :: ts) (overlay cs (env_singleton (length ts) c)).
+
+  Lemma interpret_env_free_name:
+    forall g a,
+    interpret_env g a ->
+    forall n,
+    n >= length g ->
+    ~has_free_name a n.
+  Proof.
+    induction 1; simpl; intros.
+    - intros (t, ?).
+      inversion H0.
+    - intros (u, ?).
+      unfold env_singleton, env_type in H2.
+      dependent destruction H2.
+      + eapply IHinterpret_env with n.
+        * lia.
+        * now exists u.
+      + dependent destruction H2.
+        lia.
+  Qed.
+
+  Lemma interpretation_preserves_typing:
+    forall b p,
+    interpret b p ->
+    forall g a,
+    TypeSystem.typing g b void ->
+    interpret_env g a ->
+    Control.typing O p a (length g).
+  Proof.
+    induction 1; intros.
+    - admit.
+    - dependent destruction H3.
+      unfold local_env.
+      eapply typing_iso.
+      + apply typing_res.
+        * eapply typing_par.
+          --- apply IHinterpret1 with (g := negation ts :: g).
+              +++ assumption.
+              +++ constructor; eauto.
+                  econstructor; eauto.
+          --- apply typing_in with (g := a).
+              +++ admit.
+              +++ replace (i2l (1 + length g) 0) with (length g) by lia.
+                  apply interpret_env_free_name with g.
+                  *** assumption.
+                  *** lia.
+              +++ now apply interpret_forall_generates_output with ts.
+          --- admit.
+          --- constructor.
+        * admit.
+        * admit.
+      + admit.
+  Admitted.
 
 End Interpretation.
